src/RqRsLang.v
@@ -51,6 +51,19 @@ Definition getFirstNatMsg {oifc} (st: StateM oifc): option nat :=
            | _ => None
            end).
 
+Definition UpLockMsgId {oifc} (mty: bool) (mid: IdxT): OPrec oifc :=
+  fun ost orq mins =>
+    (orq@[upRq])
+      >>=[False]
+      (fun rqiu =>
+         rqiu.(rqi_msg).(msg_type) = mty /\
+         rqiu.(rqi_msg).(msg_id) = mid).
+
+Definition getUpLockMsgId {oifc} (st: StateM oifc): option (bool * IdxT) :=
+  ((snd (fst st))@[upRq])
+    >>= (fun rqiu => Some (rqiu.(rqi_msg).(msg_type),
+                           rqiu.(rqi_msg).(msg_id))).
+
 Definition UpLockNatMsg {oifc}: OPrec oifc :=
   fun ost orq mins =>
     (orq@[upRq])
@@ -127,7 +140,9 @@ Definition MsgsTo {oifc} (tos: list IdxT) (rule: Rule oifc): Prop :=
 
 Hint Unfold StateMBind TrsMTrs getFirstMsg
      FirstNatMsg getFirstNatMsg
-     UpLockNatMsg getUpLockNatMsg UpLocked getUpLockIdxBack
+     UpLockNatMsg getUpLockNatMsg
+     UpLockMsgId getUpLockMsgId
+     UpLocked getUpLockIdxBack
      DownLockNatMsg getDownLockNatMsg DownLocked getDownLockIdxBack
      MsgsFrom MsgIdsFrom MsgsFromORq MsgsFromRsUp MsgsTo : RuleConds.
 
@@ -154,6 +169,29 @@ Module RqRsNotations.
        rule_precond := PREC%prec;
        rule_trs := TRS%trs |} (at level 5).
 End RqRsNotations.
+
+Definition AtomicMsgOutsInv {oifc} (mp: MsgOutPred oifc)
+           (eouts: list (Id Msg)) (nst: MState oifc): Prop :=
+  Forall (fun eout => mp eout nst.(bst_oss) nst.(bst_orqs)) eouts.
+
+Definition AtomicLocksInv {oifc}
+           (lp: IdxT -> ORq Msg -> Prop)
+           (hst: MHistory) (nst: MState oifc): Prop :=
+  forall oidx,
+    In oidx (oindsOf hst) ->
+    (bst_orqs nst)@[oidx] >>=[False] (fun orq => lp oidx orq).
+
+Definition AtomicInv {oifc}
+           (mp: MsgOutPred oifc)
+           (lp: IdxT -> ORq Msg -> Prop):
+  list (Id Msg) (* inits *) ->
+  MState oifc (* starting state *) ->
+  MHistory (* atomic history *) ->
+  list (Id Msg) (* eouts *) ->
+  MState oifc (* ending state *) -> Prop :=
+  fun inits st1 hst eouts st2 =>
+    AtomicMsgOutsInv mp eouts st2 /\
+    AtomicLocksInv lp hst st2.
 
 Ltac disc_rule_conds_const_unit :=
   match goal with
@@ -231,6 +269,17 @@ Ltac disc_rule_conds_const :=
           try disc_rule_conds_const_unit;
           subst; simpl in * ).
 
+Ltac disc_minds_const :=
+  repeat
+    match goal with
+    | [H: rqEdgeUpFrom ?dtr ?oidx = Some ?midx |- _] =>
+      is_const dtr; is_const oidx; is_var midx; inv H
+    | [H: rsEdgeUpFrom ?dtr ?oidx = Some ?midx |- _] =>
+      is_const dtr; is_const oidx; is_var midx; inv H
+    | [H: edgeDownTo ?dtr ?oidx = Some ?midx |- _] =>
+      is_const dtr; is_const oidx; is_var midx; inv H
+    end.
+
 Ltac solve_rule_conds_const :=
   repeat
     (repeat (autounfold with RuleConds in *; dest); intros;
@@ -255,6 +304,134 @@ Ltac rule_rqdd := do 2 right; left; split; [|right; right].
 Ltac rule_rsdd := do 3 right; left; split; [left|].
 Ltac rule_rsu := do 3 right; left; split; [right|].
 Ltac rule_rsrq := do 4 right.
+
+Ltac disc_AtomicInv :=
+  repeat
+    match goal with
+    | [H: AtomicInv _ _ _ _ _ _ _ |- _] => red in H; dest
+    end.
+
+Ltac atomic_cont_exfalso_bound msgOutPred :=
+  exfalso;
+  disc_rule_conds_ex;
+  repeat 
+    match goal with
+    | [H1: AtomicMsgOutsInv _ ?eouts _, H2: In _ ?eouts |- _] =>
+      red in H1; rewrite Forall_forall in H1;
+      specialize (H1 _ H2); simpl in H1
+    | [H: msgOutPred _ _ _ |- _] => red in H
+    | [H1: caseDec _ ?sig _ _ |- _] =>
+      match sig with
+      | sigOf (?midx, ?msg) =>
+        match goal with
+        | [H2: msg_id ?msg = ?mid, H3: msg_type ?msg = ?mty |- _] =>
+          progress replace sig with (midx, (mty, mid)) in H1
+            by (unfold sigOf; simpl; rewrite H2, H3; reflexivity);
+          simpl in H1
+        end
+      end
+    end;
+  assumption.
+
+Ltac atomic_init_exfalso_rq :=
+  exfalso;
+  disc_rule_conds_ex;
+  repeat
+    match goal with
+    | [H: _ = _ \/ _ |- _] =>
+      destruct H; [subst; try discriminate|auto]
+    end.
+
+Ltac atomic_init_exfalso_rs_from_parent :=
+  exfalso;
+  repeat
+    (repeat match goal with
+            | [H: UpLockInvORq _ _ _ _ _ |- _] => red in H
+            | [H1: ?orq@[0] = Some _, H2: context[?orq@[0]] |- _] =>
+              rewrite H1 in H2; simpl in H2
+            | [H: UpLockRsFromParent _ _ _ |- _] =>
+              let rsFrom := fresh "rsFrom" in
+              destruct H as [rsFrom [? ?]]
+            end;
+     disc_rule_conds_ex);
+  repeat
+    match goal with
+    | [H1: _ = ?rsFrom \/ _, H2: edgeDownTo _ _ = Some ?rsFrom |- _] =>
+      destruct H1; [subst; try discriminate|auto]
+    end.
+
+Ltac atomic_init_solve_AtomicMsgOutsInv :=
+  simpl; repeat constructor.
+
+Ltac atomic_init_solve_AtomicLocksInv :=
+  red; intros; dest_in;
+  repeat (simpl; mred);
+  unfold sigOf; simpl;
+  repeat
+    match goal with
+    | [H: msg_id ?msg = _ |- context [msg_id ?msg] ] => rewrite H
+    | [H1: msg_id ?msg = _, H2: context [msg_id ?msg] |- _] =>
+      rewrite H1 in H2
+    | [H: ?orq@[?i] = Some _ |- context [?orq@[?i]] ] => rewrite H
+    | [H1: ?orq@[?i] = Some _, H2: context [?orq@[?i]] |- _] =>
+      rewrite H1 in H2
+    | [H: ?orq@[?i] = None |- context [?orq@[?i]] ] => rewrite H
+    | [H1: ?orq@[?i] = None, H2: context [?orq@[?i]] |- _] =>
+      rewrite H1 in H2
+    end;
+  repeat (red; simpl; mred; auto).
+
+Ltac atomic_init_solve_AtomicInv :=
+  split; [atomic_init_solve_AtomicMsgOutsInv
+         |atomic_init_solve_AtomicLocksInv].
+
+Ltac disc_lock_preds_with Hl oidx :=
+  match type of Hl with
+  | AtomicLocksInv _ ?hst _ =>
+    match goal with
+    | [Hin: In oidx (oindsOf ?hst) |- _] =>
+      specialize (Hl _ Hin); simpl in Hl;
+      disc_rule_conds_ex; red in Hl; simpl in Hl
+    end
+  end.
+
+Ltac disc_lock_preds oidx :=
+  match goal with
+  | [H: AtomicLocksInv _ _ _ |- _] =>
+    let Hl := fresh "H" in
+    pose proof H as Hl;
+    disc_lock_preds_with Hl oidx
+  end.
+
+Ltac disc_sig_caseDec :=
+  match goal with
+  | [H1: caseDec _ ?sig _ _ |- _] =>
+    match sig with
+    | sigOf (?midx, ?msg) =>
+      match goal with
+      | [H2: msg_id ?msg = ?mid, H3: msg_type ?msg = ?mty |- _] =>
+        progress replace sig with (midx, (mty, mid)) in H1
+          by (unfold sigOf; simpl; rewrite H2, H3; reflexivity);
+        simpl in H1
+      end
+    end
+  end.
+
+Ltac disc_msg_preds_with Hl Hin :=
+  match type of Hl with
+  | AtomicMsgOutsInv _ ?eouts _ =>
+    red in Hl; rewrite Forall_forall in Hl;
+    specialize (Hl _ Hin); simpl in Hl;
+    red in Hl; disc_sig_caseDec
+  end.
+
+Ltac disc_msg_preds Hin :=
+  match goal with
+  | [H: AtomicMsgOutsInv _ _ _ |- _] =>
+    let Hl := fresh "H" in
+    pose proof H as Hl;
+    disc_msg_preds_with Hl Hin
+  end.
 
 Close Scope list.
 Close Scope hvec.
